finished blood and donordb

projectVampire/python/blood.py
@@ -1,59 +1,66 @@
 from datetime import datetime,timedelta
-
+from time_sec import time_sec
 class blood:
+    # unsafe = -1
     # unverified = 0
     # verified = 1
     # storage = 2
-    # dispatch
+    # dispatch = 3
     # delivered = 4
-    # unsafe = 5
+    
+    SECS_IN_DAY = 86400
+    BLOOD_LIFETIME = 42 * SECS_IN_DAY
 
-    def __init__(self):
+    def __init__(self,seconds_in):
         self._state = 0
-        self._collection_time=datetime.now() #=Current system time
+        self._collection_time=seconds_in
+        self._expiry_time=self._collection_time+(BLOOD_LIFETIME)
 
     def get_state(self):
         return self._state
 
     # Functions like a predicate.
-    # Returns false if either the state is invalid. (Something has gone wrong somewhere so don't trust the blood)
-    # OR the blood is due to expire in the next 25 hours.
+    # Returns false if the state is invalid. (Something has gone wrong somewhere so don't trust the blood
     def valid(self):
-        if not 0<= self._state <=5:
-            return False
-        if (self._collection_time+datetime.timedelta(days=40,hours=23)>datetime.now()):
+        if not -1<= self._state <=4:
             return False
         
+    def expired(self,curr_time):
+        return curr_time>self._expiry_time
 
-    def verify_blood(self,blood_type,rhesus):
-        if (valid()):
+    def safe(self,curr_time):
+        return 0<=self._state<=4 and not self.expired(curr_time)
+
+    # All transition methods accept curr_time as an int
+    def verify_blood(self,curr_time,blood_type,rhesus):
+        if (valid() and safe(curr_time)):
             if self._state == 0:
                 self._state = 1
                 self._type=blood_type
                 self._rhesus = rhesus
         else:
-            self._state=5
+            self._state=-1
 
-    def store_blood(self):
-        if (valid()):
+    def store_blood(self,curr_time):
+        if (valid() and safe(curr_time)):
             if self._state == 1:
                 self._state = 2
         else:
-            self._state=5
+            self._state=-1
 
-    def dispatch_blood(self):
-        if (valid()):
+    def dispatch_blood(self,curr_time):
+        if (valid() and safe(curr_time)):
             if self._state == 2:
                 self._state = 3
         else:
-            self._state=5
+            self._state=-1
 
-    def deliver_blood(self):
-        if (valid()):
+    def deliver_blood(self,curr_time):
+        if (valid() and safe(curr_time)):
             if self._state == 3:
                 self._state = 4
         else:
-            self._state=5
+            self._state=-1
     
     def get_blood_type(self):
         if self._state>=1 and self._state<=4:
@@ -61,4 +68,4 @@ class blood:
 
     # Rejection of blood for any reason - rejected by pathology, lost, expired
     def reject_blood(self):
-        self._state = 5
+        self._state = -1
