projectVampire/python/donordb.py
@@ -1,0 +1,17 @@
+from blood import blood
+
+class donor_db:
+
+    def __init__(self):
+        self._last_donation=0
+
+    def donation_allowed(self,curr_time):
+        return ((curr_time-self._last_donation)/86400)>=7
+
+    def collect_blood(self,curr_time):
+        if (self.donation_allowed(curr_time)):
+            self._last_donation=curr_time
+            return blood(curr_time)
+
+
+    
