projectVampire/python/time_sec.py
@@ -1,0 +1,22 @@
+import datetime
+class time_sec:
+
+    time_0 = datetime.datetime.utcfromtimestamp(0)
+
+    @staticmethod
+    def get_seconds(time_in):
+        diff = (time_in - time_0)
+        return diff.total_seconds()
+    
+    @staticmethod
+    def get_now():
+        return get_seconds(datetime.datetime.now())
+
+    # Returns the number of full days.
+    @staticmethod
+    def day_diff(time_1,time_2):
+        if (time_1>=time_2):
+            diff = time_1-time_2
+            days = diff/86400 # 86400 is number of seconds in a day
+            return int(days)
+
