projectVampire/dafny/time_sec.dfy
@@ -1,0 +1,18 @@
+class time_sec{
+
+    var time_0:int;
+
+    static method get_seconds(time_in:int) {
+        diff := (time_in - time_0)
+        diff
+    }
+
+    # Returns the number of full days.
+    @staticmethod
+    def day_diff(time_1,time_2):
+        if (time_1>=time_2):
+            diff = time_1-time_2
+            days = diff/86400 # 86400 is number of seconds in a day
+            return int(days)
+}
+
